@prefix sz:       <https://github.com/senzing-garage/sz-semantics/wiki/ns#> .

@prefix adms:     <http://www.w3.org/ns/adms#> .
@prefix bods:     <https://vocab.openownership.org/terms#> .
@prefix dc:       <http://purl.org/dc/elements/1.1/> .
@prefix dcat:     <http://www.w3.org/ns/dcat#> .
@prefix dcterms:  <http://purl.org/dc/terms/> .
@prefix foaf:     <http://xmlns.com/foaf/0.1/> .
@prefix ftm:      <https://schema.followthemoney.tech/#> .
@prefix nc:       <http://release.niem.gov/niem/niem-core/5.0/#> .
@prefix owl:      <http://www.w3.org/2002/07/owl#> .
@prefix ppcl:     <http://www.semantic-web.at/ppcl/> .
@prefix prov:     <http://www.w3.org/ns/prov#> .
@prefix rad:      <http://www.w3.org/ns/rad#> .
@prefix rdf:      <http://www.w3.org/1999/02/22-rdf-syntax-ns#> .
@prefix rdfs:     <http://www.w3.org/2000/01/rdf-schema#> .
@prefix skos:     <http://www.w3.org/2004/02/skos/core#> .
@prefix void:     <http://rdfs.org/ns/void#> .
@prefix wco:      <https://id.oclc.org/worldcat/ontology/> .
@prefix wd:       <http://www.wikidata.org/entity/> .
@prefix xsd:      <http://www.w3.org/2001/XMLSchema#> .

<https://contextually.poolparty.biz/senzing> a void:Dataset ;
  ppcl:numberOfConcepts "4"^^xsd:int ;
  ppcl:numberOfConceptSchemes "1"^^xsd:int ;
  ppcl:availablelanguages "fr", "es", "en" ;
  dcterms:creator <https://contextually.poolparty.biz/user/3d5c61e1-814a-43f8-8695-6afd519c37eb> ;
  dcterms:language "en" ;
  dcterms:date "2025-10-31T00:31:37.343Z"^^xsd:dateTime ;
  dcterms:title "senzing"@en ;
  void:sparqlEndpoint <https://contextually.poolparty.biz/PoolParty/sparql/senzing> ;
  void:feature _:node2 ;
  void:vocabulary <http://www.w3.org/2004/02/skos/core#> ;
.

_:node2 a void:TechnicalFeature ;
  rdfs:label "RDF/XML" ;
  dcterms:format "application/rdf+xml" ;
.

<https://contextually.poolparty.biz/senzing/adms/0.1> a adms:SemanticAsset ;
  dcterms:title "senzing"@en ;
  dcterms:created "2025-10-31T00:31:37.343Z"^^xsd:dateTime ;
  dcterms:identifier <urn:uuid:2f690379-0d7d-4d5e-877d-a7880c240856> ;
  foaf:homepage <https://contextually.poolparty.biz/PoolParty/wiki/senzing> ;
  rad:version 1.0E-1 ;
.

sz:SenzingScheme a skos:ConceptScheme ;
  dcterms:title "Resource"@en ;
  skos:definition "A mid-level SKOS taxonomy used for representing Senzing results"@en ;
  skos:hasTopConcept sz:Entity, sz:Organization, sz:Person, sz:DataRecord ;
  skos:prefLabel "Senzing minimal SKOS taxonomy"@en ;
  dcterms:publisher <https://senzing.com/> ;
  dcterms:creator <https://orcid.org/0000-0003-3167-1539> ;
.

sz:Entity a skos:Concept, nc:EntityType ;
  owl:equivalentClass ftm:LegalEntity, bods:EntityType, wco:Agent, foaf:Agent ;
  dc:identifier wd:Q35120 ;
  skos:definition "Entity is anything that can be considered, discussed, or observed ; in this context, this is generally a Person or Organization"@en ;
  skos:inScheme sz:SenzingScheme ;
  skos:topConceptOf sz:SenzingScheme ;
  skos:prefLabel "Entity"@en ;
  sz:lemma_phrase "NOUN.entity"@en ;
.

sz:Organization a skos:Concept, nc:OrganizationType ;
  rdfs:subClassOf sz:Entity ;
  owl:equivalentClass ftm:Organization, wco:Organization, foaf:Organization ;
  dc:identifier wd:Q43229 ;
  skos:definition "Organization is a social entity established to meet needs or pursue goals"@en ;
  skos:inScheme sz:SenzingScheme ;
  skos:topConceptOf sz:SenzingScheme ;
  skos:prefLabel "Organization"@en ;
  sz:lemma_phrase "NOUN.organization"@en ;
  sz:ner_label true ;
.

sz:Person a skos:Concept, nc:PersonType ;
  rdfs:subClassOf sz:Entity ;
  owl:equivalentClass ftm:Person, bods:PersonType, wco:Person, foaf:Person ;
  dc:identifier wd:Q5 ;
  skos:definition "Person represents an individual human being, distinct from some type of corporation, which may encompass real or deceased people, or their pseudonyms"@en ;
  skos:inScheme sz:SenzingScheme ;
  skos:topConceptOf sz:SenzingScheme ;
  skos:prefLabel "Person"@en ;
  sz:lemma_phrase "NOUN.person"@en ;
  sz:ner_label true ;
.

sz:DataRecord a skos:Concept ;
  owl:equivalentClass prov:Entity, bods:RecordDetails, wco:TransactionalEvent ;
  dc:identifier wd:Q2470517 ;
  skos:definition "Data Record is a composite data type, as an information block containing specific, identified fields"@en ;
  skos:inScheme sz:SenzingScheme ;
  skos:topConceptOf sz:SenzingScheme ;
  skos:prefLabel "Data Record"@en ;
  skos:altLabel "Record"@en ;
  sz:lemma_phrase "NOUN.data NOUN.record"@en ;
.


sz:relation a rdf:Property .

sz:match_key rdfs:subPropertyOf sz:relation ;
  rdfs:domain sz:Entity ;
  rdfs:range xsd:string ;
  skos:definition "indicates which features matched when a data record was last processed individually"@en ;
.

sz:match_level a sz:relation ;
  rdfs:domain sz:Entity ;
  rdfs:range xsd:string ;
  skos:definition "describes how the source data record contributes to this entity"@en ;
.

sz:lemma_phrase rdfs:subPropertyOf sz:relation ;
  rdfs:domain skos:Concept ;
  rdfs:range rdf:langString ;
  skos:definition "a parsed, lemmatized noun phrase, used as a unique identifier in entity linking"@en ;
.

sz:ner_label rdfs:subPropertyOf sz:relation ;
  rdfs:domain skos:Concept ;
  rdfs:range xsd:boolean ;
  skos:definition "indicates whether the skos:prefLabel value can be used as an NER label"@en ;
.

sz:member_of rdfs:subPropertyOf sz:relation ;
  owl:equivalentClass wco:memberOf ;
  rdfs:domain sz:Person ;
  rdfs:range sz:Organization ;
  skos:definition "indicates when a person is known to be a member of an organization"@en ;
.
