@prefix sz:    <https://github.com/senzing-garage/sz-semantics/wiki/ns#> .

@prefix bods:  <https://vocab.openownership.org/terms#> .
@prefix dc:    <http://purl.org/dc/elements/1.1/> .
@prefix dcat:  <http://www.w3.org/ns/dcat#> .
@prefix ftm:   <https://schema.followthemoney.tech/#> .
@prefix prov:  <http://www.w3.org/ns/prov#> .
@prefix rdf:   <http://www.w3.org/1999/02/22-rdf-syntax-ns#> .
@prefix rdfs:  <http://www.w3.org/2000/01/rdf-schema#> .
@prefix skos:  <http://www.w3.org/2004/02/skos/core#> .
@prefix wco:   <https://id.oclc.org/worldcat/ontology/> .
@prefix wd:    <http://www.wikidata.org/entity/> .
@prefix xsd:   <http://www.w3.org/2001/XMLSchema#> .


sz:match_key rdfs:domain sz:Entity ;
  rdfs:range xsd:string ;
  skos:definition "which features matched when a record last was processed individually"@en
.

sz:match_level rdfs:domain sz:Entity ;
  rdfs:range xsd:integer ;
  skos:definition "signifies how the source record contributes to this entity"@en
.

sz:lemma_phrase rdfs:domain skos:Concept ;
  rdfs:range rdf:langString ;
  skos:definition "the parsed, lemmatized noun phrase for an extracted entity"@en
.

sz:member_of rdfs:domain sz:Person ;
  rdfs:range sz:Organization ;
  skos:definition "which people are members of which organizations?"@en ;
  rdf:type sz:relation, wco:memberOf
.


sz:SenzingScheme rdf:type skos:ConceptScheme ;
  dc:publisher <https://senzing.com/> ;
  dc:creator <https://orcid.org/0000-0003-3167-1539> ;
  skos:definition "A mid-level SKOS taxonomy used for representing Senzing results"@en ;
  skos:prefLabel "Senzing minimal SKOS taxonomy"@en
 .

sz:Entity rdf:type skos:Concept , bods:Entity , ftm:LegalEntity , wco:Agent ;
 skos:inScheme sz:SenzingScheme ;
 skos:topConceptOf sz:SenzingScheme ;
 skos:prefLabel "Entity"@en ;
 sz:lemma_phrase "NOUN.entity"@en ;
 skos:definition "An Entity is anything that can be considered, discussed, or observed; in this context, this is generally a Person or Organization"@en ;
 dc:identifier wd:Q35120
.

sz:DataRecord rdf:type skos:Concept , prov:Entity , wco:TransactionalEvent ;
 skos:inScheme sz:SenzingScheme ;
 skos:topConceptOf sz:SenzingScheme ;
 skos:prefLabel "Data Record"@en ;
 skos:altLabel "Record"@en ;
 sz:lemma_phrase "NOUN.data NOUN.record"@en ;
 skos:definition "A Data Record is a composite data type; an information block containing specific, identified fields"@en ;
 dc:identifier wd:Q2470517
.

sz:Person rdf:type skos:Concept , bods:Person , ftm:Person , wco:Person ;
 skos:inScheme sz:SenzingScheme ;
 rdfs:subClassOf sz:Entity ;
 skos:prefLabel "Person"@en ;
 sz:lemma_phrase "NOUN.person"@en ;
 skos:definition "A Person is any single member of Homo sapiens, unique extant species of the genus Homo"@en ;
 dc:identifier wd:Q5
.

sz:Organization rdf:type skos:Concept , ftm:Organization , wco:Organization ;
 skos:inScheme sz:SenzingScheme ;
 rdfs:subClassOf sz:Entity ;
 skos:prefLabel "Organization"@en ;
 sz:lemma_phrase "NOUN.organization"@en ;
 skos:definition "An Organization is a social entity established to meet needs or pursue goals"@en ;
 dc:identifier wd:Q43229
.
